Finish proc_interp_strong_confl_at_mod

Wavelet/Semantics/PCM.lean
@@ -8,36 +8,58 @@ class PCM (C : Type u) where
   valid : C → Prop
   eq : C → C → Prop
 
-infixl:60 " ⊔ " => PCM.add
-infix:40 " ≡ " => PCM.eq
-prefix:40 "✓ " => PCM.valid
+namespace PCM
 
-def PCM.disjoint [PCM C] (a b : C) : Prop := ✓ a ⊔ b
+infixl:60 " ⊔ " => add
+infix:40 " ≡ " => eq
+prefix:40 "✓ " => valid
 
-def PCM.framePreserving [PCM C] (a b : C) : Prop :=
+def disjoint [PCM C] (a b : C) : Prop := ✓ a ⊔ b
+
+def framePreserving [PCM C] (a b : C) : Prop :=
   ∀ c, ✓ a ⊔ c → ✓ b ⊔ c
 
-def PCM.sum [PCM C] (xs : List C) : C :=
-  xs.foldl (· ⊔ ·) PCM.zero
+def sum [PCM C] (xs : List C) : C :=
+  xs.foldl (· ⊔ ·) zero
 
-infix:50 " ⊥ " => PCM.disjoint
-infix:50 " ⟹ " => PCM.framePreserving
+infix:50 " ⊥ " => disjoint
+infix:50 " ⟹ " => framePreserving
 
 instance [PCM C] : LE C where
   le a b := ∃ c, b ≡ a ⊔ c
 
-noncomputable def PCM.sub [PCM C] (a b : C) (hle : b ≤ a) : C :=
+noncomputable def sub [PCM C] (a b : C) (hle : b ≤ a) : C :=
   hle.choose
 
-class LawfulPCM (R : Type u) [inst : PCM R] where
-  add_comm : ∀ a b : R, a ⊔ b ≡ b ⊔ a
-  add_assoc : ∀ a b c : R, (a ⊔ b) ⊔ c ≡ a ⊔ (b ⊔ c)
-  add_ident : ∀ a : R, a ⊔ inst.zero ≡ a
-  valid_add : ∀ a b : R, ✓ a ⊔ b → ✓ a
+class Lawful (R : Type u) [inst : PCM R] where
+  add_comm : ∀ {a b : R}, a ⊔ b ≡ b ⊔ a
+  add_assoc : ∀ {a b c : R}, (a ⊔ b) ⊔ c ≡ a ⊔ (b ⊔ c)
+  add_ident : ∀ {a : R}, a ⊔ inst.zero ≡ a
+  valid_add : ∀ {a b : R}, ✓ a ⊔ b → ✓ a
   valid_zero : ✓ inst.zero
-  valid_eq : ∀ a b : R, a ≡ b → ✓ a → ✓ b
-  eq_refl : ∀ a : R, a ≡ a
-  eq_symm : ∀ a b : R, a ≡ b → b ≡ a
-  eq_trans : ∀ a b c : R, a ≡ b → b ≡ c → a ≡ c
+  valid_eq : ∀ {a b : R}, a ≡ b → ✓ a → ✓ b
+  eq_refl : ∀ {a : R}, a ≡ a
+  eq_symm : ∀ {a b : R}, a ≡ b → b ≡ a
+  eq_trans : ∀ {a b c : R}, a ≡ b → b ≡ c → a ≡ c
+  eq_congr_add :
+    ∀ {a₁ a₂ b₁ b₂ : R},
+      a₁ ≡ a₂ →
+      b₁ ≡ b₂ →
+      a₁ ⊔ b₁ ≡ a₂ ⊔ b₂
+
+theorem eq_congr_disj
+  [PCM C] [Lawful C]
+  {a₁ a₂ b₁ b₂ : C}
+  (ha : a₁ ≡ a₂)
+  (hb : b₁ ≡ b₂)
+  (hdisj : a₁ ⊥ b₁) :
+    a₂ ⊥ b₂
+  := by
+  simp [disjoint]
+  apply Lawful.valid_eq
+  apply Lawful.eq_congr_add ha hb
+  exact hdisj
+
+end PCM
 
 end Wavelet.Semantics
